A first implementation with type conversions from C11-AST

C11-BackEnds/Clean_wrapper/examples/Coder_Example_1.thy
@@ -2,7 +2,7 @@ theory "Coder_Example_1"
   imports "../src/CleanCoder"
 begin
 
-section \<open>converters\<close>
+section \<open>Library and C-Env Stuff\<close>
 
 ML\<open>
 fun map_option f (SOME X) = SOME(f X)
@@ -13,76 +13,25 @@ fun lookup_Cid_info (C_env:C_Module.Data_In_Env.T) id = Symtab.lookup(#idents(#v
 
 fun is_global_Cid Cenv Cid   = map_option (fn (_,_,X) => #global X) (lookup_Cid_info Cenv Cid);
 fun is_fun_Cid Cenv Cid      = map_option (fn (_,_,X) => [] <> #params X) (lookup_Cid_info Cenv Cid);
+    (* this is wrong in general !!! [CFunDeclr0 *)
 fun get_CDeclSpecS_Cid Cenv id= map_option (fn (_,_,X) => #ret X) (lookup_Cid_info Cenv id);
 
-fun conv_ParseStatus_CDeclSpecS (SOME(C_Env.Parsed S)) = SOME S
-   |conv_ParseStatus_CDeclSpecS _ = NONE
 
 \<close>
-section \<open>expressions\<close>
 
-text \<open>
-First, we translate the expressions;
-we can have binary operators, unary operators, or constants.
-The attributs can be constantes or variables. 
-In order to simulate the use of variables, we construct a "fake" record local_state
-\<close>
-
-global_vars test  (*intern label *)
-            a     :: "int"
-
-ML\<open>val Const(longid_a,Type("fun",[sigma_i, _])) = @{term "a"} \<close>
-
-declare [[C\<^sub>r\<^sub>u\<^sub>l\<^sub>e\<^sub>0 = "translation_unit"]]
-declare [[C\<^sub>e\<^sub>n\<^sub>v\<^sub>0 = last]]
-
-C\<open> int a[10+12][34][] = 1;
-   int f(short int x [], long double y);
-\<close>
-
-ML\<open>val env_expr : C_Module.Data_In_Env.T =  @{C\<^sub>e\<^sub>n\<^sub>v};\<close>
-
-ML\<open>
-   val SOME(pos_list,ser,S)    = lookup_Cid_info env_expr "a";
-   val SOME(pos_list',ser',S') = lookup_Cid_info env_expr "f";
-\<close>
+section \<open>converters for C-types\<close>
 
 ML\<open>
 local open C_Ast C_Env in
 
-(*
-fold (fn C_Ast.CArrDeclr0 _ => (fn tyf => HOLogic.listT o tyf)
-        |C_Ast.CFunDeclr0 _ => (fn tyf => curry (op -->) tyf)
-        | _ => error "non-convertible C-type")
-*)
-val _ = C_Ast.CTypeSpec0 : 'a C_Ast.cTypeSpecifier ->  'a C_Ast.cDeclarationSpecifier;
-val _ = C_Ast.CFunDeclr0;
-val _ = C_Ast.Right
-val [CArrDeclr0 (HH,CArrSize0 (_,CBinary0 X),_),
-     CArrDeclr0 (_,CArrSize0  (_,CConst0 Y), _), 
-     CArrDeclr0 (_,CNoArrSize0 Z,_)] = #params S
-val [CFunDeclr0 (Right([CDecl0 (A, A',_),CDecl0 (B,B',_)],s), _, _)] = #params S'
-
-end
-\<close>
-
-ML\<open>
-fold_rev (fn C_Ast.CDecl0 (A, _ ,_) => fn S => (SOME A) :: S) ;
-A;
-B;
-\<close>
-ML\<open>
-local open C_Ast C_Env in
-
-(* mk_CFunDeclr0; *)
-(*val CSpec = (get_CDeclSpecS_Cid env_expr "a"); *)
-val CTypeSpec = conv_ParseStatus_CDeclSpecS (get_CDeclSpecS_Cid env_expr "a");
-val CTypeSpec' = conv_ParseStatus_CDeclSpecS (get_CDeclSpecS_Cid env_expr "f");
 (*
   and 'a cTypeSpecifier = CVoidType0 of 'a | CCharType0 of 'a | CShortType0 of 'a 
                        | CIntType0 of 'a | CLongType0 of 'a | CFloatType0 of 'a 
                        | CDoubleType0 of 'a | CSignedType0 of 'a | CUnsigType0 of 'a | CBoolType0 of 'a |
 *)
+fun conv_ParseStatus_CDeclSpecS (SOME(C_Env.Parsed S)) = SOME S
+   |conv_ParseStatus_CDeclSpecS _ = NONE
+
 fun conv_cDeclarationSpecifier_typ (SOME([CTypeSpec0 (CUnsigType0 _)])) = SOME(HOLogic.intT)
    |conv_cDeclarationSpecifier_typ (SOME([CTypeSpec0 (CIntType0 _)]))   = SOME(HOLogic.intT)
    |conv_cDeclarationSpecifier_typ (SOME([CTypeSpec0 (CLongType0 _),
@@ -110,14 +59,14 @@ fun conv_cDeclarationSpecifier_typ (SOME([CTypeSpec0 (CUnsigType0 _)])) = SOME(H
 
 fun conv_cDerivedDeclarator_cArraySize_term (CArrDeclr0 (_,CArrSize0 (_,C_expr),_)) C_env thy = 
             SOME(hd((C11_Ast_Lib.fold_cExpression 
-                               (convertExpr_raw false sigma_i C_env thy) C_expr [])))
+                               (convertExpr_raw false dummyT C_env thy) C_expr [])))
    |conv_cDerivedDeclarator_cArraySize_term (CArrDeclr0 (_,CNoArrSize0 Z,_)) _ _ =NONE
    |conv_cDerivedDeclarator_cArraySize_term (_)  _ _ = 
             error("Derived declarator format not defined. [Clean restriction]")
 
 fun conv_cDerivedDeclarator_cSizeExpr_term (CArrDeclr0 (_,CArrSize0 (_,C_expr),_)) C_env thy = 
             SOME(hd((C11_Ast_Lib.fold_cExpression 
-                                 (convertExpr_raw false sigma_i C_env thy) C_expr [])))
+                                 (convertExpr_raw false dummyT C_env thy) C_expr [])))
    |conv_cDerivedDeclarator_cSizeExpr_term (CArrDeclr0 (_,CNoArrSize0 Z,_)) _ _ = NONE
    |conv_cDerivedDeclarator_cSizeExpr_term (_)  _ _ =  
             error("DeclarationSpec format not defined. [Clean restriction]")
@@ -127,18 +76,73 @@ fun conv_cDerivedDeclarator_typS (CArrDeclr0 (_,CArrSize0 _ ,_)) C_env thy = HOL
                     (*no enumerations ? nat ? *)
    |conv_cDerivedDeclarator_typS (CFunDeclr0 (Right(S,_), _, _)) C_env thy = I
 
+fun conv_CDerivedDecl_typ [CFunDeclr0 (Right(SS,_), _, _)] = 
+        fold_rev (fn CDecl0 (A, _ ,_) => (fn S => the (conv_cDeclarationSpecifier_typ(SOME A)) --> S)
+                     | _ => error "CDerivedDecl (0) format not defined. [Clean restriction]") SS 
+   |conv_CDerivedDecl_typ (S as CArrDeclr0 _ :: _) = 
+        fold     (fn (CArrDeclr0 _  ) => (fn tyF => HOLogic.listT o tyF)
+                     | _ => error "CDerivedDecl (1) format not defined. [Clean restriction]") S I 
+   |conv_CDerivedDecl_typ _ = error "CDerivedDecl (2) format not defined. [Clean restriction]"
+
+fun conv_GlobalIdDescr_typ (S:C_Env.markup_ident) = 
+    conv_CDerivedDecl_typ (#params S) 
+    ((the o conv_cDeclarationSpecifier_typ o conv_ParseStatus_CDeclSpecS o SOME) (#ret S));
+
 end;
-conv_cDeclarationSpecifier_typ CTypeSpec;
-conv_cDeclarationSpecifier_typ CTypeSpec';
-C_Ast.CFunSpec0;
-fun conv_CDecls_typS X = fold_rev (fn C_Ast.CDecl0 (A, _ ,_) => fn S => the (conv_cDeclarationSpecifier_typ (SOME A)) --> S) X ;
-val [C_Ast.CFunDeclr0 (C_Ast.Right(SS,_), _, _)] = #params S';
-conv_CDecls_typS SS HOLogic.boolT; 
 \<close>
 
-ML\<open>
-A'
+
+section \<open>expressions\<close>
+
+text \<open>
+First, we translate the expressions;
+we can have binary operators, unary operators, or constants.
+The attributs can be constantes or variables. 
+In order to simulate the use of variables, we construct a "fake" record local_state
 \<close>
+
+global_vars test  (*intern label *)
+            a     :: "int"
+
+(* creation of a global variable Clean state with "a" *)
+ML\<open>val Const(longid_a,Type("fun",[sigma_i, _])) = @{term "a"} \<close>
+
+
+(* creation of two declarations with "a" an array and "f" a function *)
+
+declare [[C\<^sub>r\<^sub>u\<^sub>l\<^sub>e\<^sub>0 = "translation_unit"]]
+declare [[C\<^sub>e\<^sub>n\<^sub>v\<^sub>0 = last]]
+
+C\<open> int a[10+12][34][] = 1;
+   int f(short int x [], long double y);
+\<close>
+
+(* binding the resulting C_Env to env_expr *)
+
+ML\<open>val env_expr : C_Module.Data_In_Env.T =  @{C\<^sub>e\<^sub>n\<^sub>v};\<close>
+
+(* messing around with the C identifier "a" and "f" *)
+
+ML\<open>
+   val SOME(pos_list,ser,S)    = lookup_Cid_info env_expr "a";
+   val SOME(pos_list',ser',S') = lookup_Cid_info env_expr "f";
+
+local open C_Ast C_Env in
+
+   val [CArrDeclr0 (HH,CArrSize0 (_,CBinary0 X),_),
+        CArrDeclr0 (_,CArrSize0  (_,CConst0 Y), _), 
+        CArrDeclr0 (_,CNoArrSize0 Z,_)] = #params S
+   val [CFunDeclr0 (Right([CDecl0 (A, A',_),CDecl0 (B,B',_)],s), _, _)] = #params S'
+
+end
+\<close>
+
+(* and the whole thing a bit more abstract with "a" and "f" *)
+ML\<open>
+map_option (conv_GlobalIdDescr_typ o #3) (lookup_Cid_info env_expr "a" );
+map_option (conv_GlobalIdDescr_typ o #3) (lookup_Cid_info env_expr "f" );
+\<close>
+
 
 (*1*****************************************************************************************************)
 
